Full proof of jellyfish (missing client)

jellyfish/code.v
@@ -16,14 +16,24 @@ End SKIP_LIST_PARAMS.
 Module SkipList (Params: SKIP_LIST_PARAMS).
   Import Params.
   
-  Definition tail : node_rep := (INT_MAX, dummy_null, dummy_null, None, dummy_lock).
+  Definition tail : node_rep := (INT_MAX, dummy_null, dummy_null, None, dummy_lock, dummy_null).
 
   (* Skip list constructor *)  
+  Definition initLocks : val := 
+    rec: "locks" "pt" "lvl" :=
+      if: "lvl" = #(MAX_HEIGHT + 1)
+      then #()
+      else 
+        "pt" +ₗ "lvl" <- newlock #();;
+        "locks" "pt" ("lvl" + #1).
+
   Definition new : val := 
     λ: "_", 
       let: "np" := ref (rep_to_node tail) in
       let: "next" := AllocN #(MAX_HEIGHT + 1) "np" in
-        ref (#INT_MIN, #dummy_null, "next", NONEV, newlock #()).
+      let: "locks" := AllocN #(MAX_HEIGHT + 1) #() in
+        initLocks "locks" #0;;
+        ref (#INT_MIN, #dummy_null, "next", NONEV, dummy_lock, "locks").
 
   (* Find function *)
   Definition find : val := 
@@ -40,7 +50,9 @@ Module SkipList (Params: SKIP_LIST_PARAMS).
       let: "pair" := find "head" "k" "lvl" in
       let: "pred" := Fst "pair" in
       let: "curr" := Snd "pair" in
-        acquire (nodeLock "pred");;
+      let: "locks" := nodeLocks "pred" in
+      let: "lock" := !("locks" +ₗ "lvl") in
+        acquire "lock";;
         let: "np" := nodeNext "pred" in
         let: "next" := ! !("np" +ₗ "lvl") in
         let: "nk" := nodeKey "next" in
@@ -48,7 +60,7 @@ Module SkipList (Params: SKIP_LIST_PARAMS).
           if: "nk" = "ck" 
           then "pair"
           else
-            release (nodeLock "pred");;
+            release "lock";;
             "find" "pred" "k" "lvl".
 
   (* Skip list lookup *)
@@ -79,10 +91,11 @@ Module SkipList (Params: SKIP_LIST_PARAMS).
       let: "np" := nodeNext "pred" in
       let: "succ" := !"np" in
       let: "next" := AllocN ("h" + #1) #() in
-      let: "val" := ref ("t", "v", #dummy_null) in
-      let: "node" := ref ("k", "val", #dummy_null, "next", NONEV, newlock #()) in
-        acquire (nodeLock !"node");;
+      let: "locks" := AllocN ("h" + #1) #() in
+      let: "val" := ref ("v", "t", #dummy_null) in
+      let: "node" := ref ("k", "val", "next", NONEV, #(), "locks") in
         "next" <- "succ";;
+        "locks" <- newlock #();;
         "np" <- "node";;
         "node".
 
@@ -91,33 +104,36 @@ Module SkipList (Params: SKIP_LIST_PARAMS).
       let: "np" := nodeNext "pred" in
       let: "succ" := !("np" +ₗ "lvl") in
       let: "next" := nodeNext !"node" in
+      let: "locks" := nodeLocks !"node" in
         ("next" +ₗ "lvl") <- "succ";;
+        ("locks" +ₗ "lvl") <- newlock #();;
         ("np" +ₗ "lvl") <- "node".
 
   (* Lazy list insertion *)
   Definition update : val := 
-    λ: "head" "k" "h",
+    λ: "curr" "v" "t",
+      let: "vp" := nodeVal "curr" in
+      let: "val" := !"vp" in
+      let: "ts" := valTs "val" in
+        if: "t" < "ts" 
+        then #()
+        else "vp" <- ("v", "t", ref "val").
+
+  Definition tryInsert : val := 
+    λ: "head" "k" "v" "t" "h",
       let: "pair" := findLock "head" "k" #0 in
       let: "pred" := Fst "pair" in
+      let: "lock" := !(nodeLocks "pred") in
       let: "curr" := Snd "pair" in
       let: "ck" := nodeKey "curr" in
         if: "k" = "ck"
         then 
-          let: "vp" := nodeVal "curr" in
-          let: "val" := !"vp" in
-          let: "ts" := valTs "val" in
-            if: "t" < "ts" 
-            then
-              release (nodeLock "pred");;
-              NONEV
-            else
-              let: "new" := ("t", "v", ref "val") in
-                "vp" <- "new";;
-                release (nodeLock "pred");;
-                NONEV
+          update "curr" "v" "t";;
+          release "lock";;
+          NONEV
         else 
           let: "node" := createAndLink "pred" "k" "v" "t" "h" in
-            release (nodeLock "pred");;
+            release "lock";;
             SOME "node".
 
   Definition insert : val := 
@@ -125,8 +141,9 @@ Module SkipList (Params: SKIP_LIST_PARAMS).
       let: "k" := nodeKey !"node" in
       let: "pair" := findLock "head" "k" "lvl" in
       let: "pred" := Fst "pair" in
+      let: "lock" := !(nodeLocks "pred" +ₗ "lvl") in
         link "pred" "lvl" "node";;
-        release (nodeLock "pred").
+        release ("lock").
 
   (* Skip list insertion *)
   Definition topLevel : val := 
@@ -142,7 +159,7 @@ Module SkipList (Params: SKIP_LIST_PARAMS).
       let: "pair" := find "head" "k" "lvl" in
       let: "pred" := Fst "pair" in
         if: "lvl" = #0
-        then update "pred" "k" "v" "t" "h"
+        then tryInsert "pred" "k" "v" "t" "h"
         else
           let: "onode" := "put" "pred" "k" "v" "t" "h" ("lvl" - #1) in
             match: "onode" with
@@ -156,10 +173,7 @@ Module SkipList (Params: SKIP_LIST_PARAMS).
     λ: "head" "k" "v" "t" "h",
       let: "np" := !"head" in
       let: "pred" := topLevel "np" "k" "h" #MAX_HEIGHT in
-      let: "onode" := putAll "pred" "k" "v" "t" "h" "h" in
-        match: "onode" with
-          NONE => #()
-        | SOME "node" => release (nodeLock !"node")
-        end.
+      let: "_" := putAll "pred" "k" "v" "t" "h" "h" in
+        #().
 
 End SkipList.
