jellyfish/inv/lazy_inv.v
@@ -9,21 +9,6 @@ From SkipList.jellyfish Require Import code.
 From SkipList.lib Require Import misc node_rep node_lt key_equiv.
 From SkipList.jellyfish Require Import list_equiv.
 
-Class gset_list_unionGS Σ := GsetGS { 
-  gset_nr_A_inGS :> inG Σ (frac_authR (gmapUR Z (arg_maxR Z)));
-  gset_nr_F_inGS :> inG Σ (authR (gsetUR node_rep));
-  gset_Z_disj_inGS :> inG Σ (gset_disjR Z)
-}.
-
-Record sub_gname := mk_sub_gname {
-  s_auth: gname;
-  s_toks: gname
-}.
-
-Record bot_gname := mk_bot_gname {
-  s_frac: gname
-}.
-
 Module LazyListInv (Params: SKIP_LIST_PARAMS).
   Import Params.
   Module ListEquiv := ListEquiv Params.
@@ -32,22 +17,10 @@ Module LazyListInv (Params: SKIP_LIST_PARAMS).
   Section Proofs.
     Context `{!heapGS Σ, !gset_list_unionGS Σ, !lockG Σ} (lvl: Z).
 
-    Definition from_sub_list (sub: sub_gname) (rep: node_rep) : iProp Σ := 
-      own (s_auth sub) (◯ {[ rep ]})
-      ∗
-      own (s_toks sub) (GSet {[ node_key rep ]}).
-
-    Definition from_bot_list (Smap: gmap Z (prodZ Z)) (rep: node_rep) : iProp Σ := 
-      ∃ (v: val_rep) (vs: gset Z), 
-        (node_val rep) ↦{#1 / 2} rep_to_val v
-        ∗
-        ⌜ Smap !! (node_key rep) = Some (vs, val_ts v) ⌝
-        ∗
-        ⌜ val_v v ∈ vs ⌝.
-
     Definition node_key_range : gset Z := Zlt_range INT_MIN INT_MAX.
 
-    Definition sub_list_inv (head: node_rep) (Γ: sub_gname) (P: node_rep → iProp Σ) 
+    Definition sub_list_inv (head: node_rep) (Γ: sub_gname) 
+      (osub: option sub_gname) (omap: option (gmap Z (argmax Z)))
       (S: gset node_rep) (Skeys: gset Z) (L: list node_rep) : iProp Σ := 
       ⌜ Permutation L (elements S) ⌝
       ∗
@@ -59,50 +32,33 @@ Module LazyListInv (Params: SKIP_LIST_PARAMS).
       ∗
       own (s_toks Γ) (GSet (node_key_range ∖ Skeys))
       ∗
-      list_equiv lvl ([head] ++ L) P.
+      list_equiv lvl osub ([head] ++ L) omap.
+
+    Definition bot_list_inv (Γ: bot_gname) (Smap: gmap Z (argmax Z)) : iProp Σ := 
+      own (s_frac Γ) (●F Smap)
+      ∗
+      own (s_keys Γ) (GSet (node_key_range ∖ (dom Smap))).
 
     Definition lazy_list_inv (head: node_rep) (bot: bot_gname)
       (top_sub: sub_gname) (obot_sub: option sub_gname) : iProp Σ := 
-      ∃ (S: gset node_rep) (Smap: gmap Z (prodZ Z)) (L: list node_rep),
-      match obot_sub with
-      | Some bot_sub => sub_list_inv head top_sub (from_sub_list bot_sub) S (dom Smap) L
-      | None => sub_list_inv head top_sub (from_bot_list Smap) S (dom Smap) L
-                ∗
-                own (s_frac bot) (●F Smap)
-      end.
+      ∃ (S: gset node_rep) (Smap: gmap Z (argmax Z)) (L: list node_rep),
+        sub_list_inv head top_sub obot_sub (opt_map obot_sub Smap) S (dom Smap) L
+        ∗
+        match obot_sub with
+        | Some bot_sub => True
+        | None => bot_list_inv bot Smap
+        end.
 
     Definition levelN (lvl: Z) := nroot .@ "level" .@ lvl.
 
     Definition is_sub_list (head: node_rep) (bot: bot_gname) (top_sub bot_sub: sub_gname) : iProp Σ := 
       inv (levelN lvl) (lazy_list_inv head bot top_sub (Some bot_sub)).
 
-    Definition is_bot_list (head: node_rep) (Smap: gmap Z (prodZ Z)) (q: frac)
+    Definition is_bot_list (head: node_rep) (Smap: gmap Z (argmax Z)) (q: frac)
       (bot: bot_gname) (sub: sub_gname) : iProp Σ := 
       own (s_frac bot) (◯F{q} Smap)
       ∗
       inv (levelN lvl) (lazy_list_inv head bot sub None).
-
-    
-    Lemma lazy_match_inv (head: node_rep) (bot: bot_gname)
-      (sub: sub_gname) (obot: option sub_gname) :
-      lazy_list_inv head bot sub obot ⊢
-        ∃ (P: node_rep → iProp Σ) (S: gset node_rep) (Skeys: gset Z) (L: list node_rep),
-          sub_list_inv head sub P S Skeys L
-          ∗
-          (sub_list_inv head sub P S Skeys L -∗ lazy_list_inv head bot sub obot).
-    Proof.
-      destruct obot as [bot_sub|].
-      + iIntros "Hsub"; unfold lazy_list_inv.
-        iDestruct "Hsub" as (S Smap L) "Hsub".
-        iExists (from_sub_list bot_sub), S, (dom Smap), L.
-        iFrame. iIntros "Hsub".
-        iExists S, Smap, L; iFrame.
-      + iIntros "Hbot"; unfold lazy_list_inv.
-        iDestruct "Hbot" as (S Smap L) "(Hsub & Hown)".
-        iExists (from_bot_list Smap), S, (dom Smap), L.
-        iFrame. iIntros "Hsub".
-        iExists S, Smap, L; iFrame.
-    Qed.
 
   End Proofs.
 End LazyListInv.
