jellyfish/inv/list_equiv.v
@@ -1,13 +1,31 @@
 From Coq Require Import Sorting.Sorted.
 
 From iris.base_logic.lib Require Import invariants.
+From iris.algebra Require Import cmra auth frac_auth gmap gset.
 From iris.heap_lang Require Import proofmode.
 
+From SkipList.lib Require Import arg_max.
 From SkipList.jellyfish Require Import code.
 From SkipList.lib Require Import misc node_rep node_lt key_equiv.
 
 
 Local Open Scope Z.
+
+Class gset_list_unionGS Σ := GsetGS { 
+  gset_nr_A_inGS :> inG Σ (frac_authR (gmapUR Z (arg_maxUR Z)));
+  gset_nr_F_inGS :> inG Σ (authR (gsetUR node_rep));
+  gset_Z_disj_inGS :> inG Σ (gset_disjR Z)
+}.
+
+Record sub_gname := mk_sub_gname {
+  s_auth: gname;
+  s_toks: gname
+}.
+
+Record bot_gname := mk_bot_gname {
+  s_frac: gname;
+  s_keys: gname
+}.
 
 Module ListEquiv (Params: SKIP_LIST_PARAMS).
   Import Params.
@@ -15,82 +33,203 @@ Module ListEquiv (Params: SKIP_LIST_PARAMS).
   Export SkipList.
 
   Section Proofs.
-    Context `{!heapGS Σ, !lockG Σ} (lvl: Z).
+    Context `{!heapGS Σ, !gset_list_unionGS Σ, !lockG Σ} (lvl: Z) (osub: option sub_gname).
 
-    Definition is_array (next: loc) (h: Z) : iProp Σ := 
-      ∃ (vs: list val), next ↦∗{#1 / 2} vs ∗ ⌜ length vs = Z.to_nat h ⌝.
+    Definition is_node (rep: node_rep) (v: val_rep) : iProp Σ :=
+      match osub with
+      | Some bot => own (s_auth bot) (◯ {[ rep ]})
+                    ∗
+                    own (s_toks bot) (GSet {[ node_key rep ]})
+                    
+      | None => (node_val rep) ↦{#1 / 2} rep_to_val v
+      end.
 
-    Fixpoint list_equiv (L: list node_rep) (P: node_rep → iProp Σ) : iProp Σ :=
+    Definition is_val (omap: option (gmap Z (argmax Z))) (rep: node_rep) (v: val_rep) : Prop :=
+      match omap with
+      | Some Smap => ∃ (vs: gset Z), Smap !! (node_key rep) = Some (prodZ vs (val_ts v))
+                                    ∧
+                                    val_v v ∈ vs
+      | None => True
+      end.
+
+    Definition locked_val (succ: node_rep) : iProp Σ := 
+      match osub with
+      | Some _ => True
+      | None => ⌜ succ = tail ⌝ 
+                ∨ 
+                ∃ (v: val_rep), (node_val succ) ↦{#1 / 2} rep_to_val v
+      end.
+
+    Definition in_lock (rep: node_rep) : iProp Σ := 
+      ∃ (s: loc) (succ: node_rep), 
+        (node_next rep +ₗ lvl) ↦{#1 / 2} #s 
+        ∗ 
+        s ↦□ rep_to_node succ
+        ∗
+        locked_val succ.
+
+    Definition opt_map (Smap: gmap Z (argmax Z)) : option (gmap Z (argmax Z)) :=
+      match osub with
+      | Some _ => None
+      | None => Some Smap
+      end.
+
+    Definition opt_lookup (omap: option (gmap Z (argmax Z))) (key: Z) : option (argmax Z) := 
+      match omap with
+      | Some Smap => Smap !! key
+      | None => None
+      end.
+
+    Definition opt_insert (omap: option (gmap Z (argmax Z))) (key: Z) (v: argmax Z) : option (gmap Z (argmax Z)) :=
+      match omap with
+      | Some Smap => Some (<[key := v]>Smap)
+      | None => None
+      end.
+
+    Definition opt_delete (omap: option (gmap Z (argmax Z))) (key: Z) : option (gmap Z (argmax Z)) :=
+      match omap with
+      | Some Smap => Some (delete key Smap)
+      | None => None
+      end.
+
+    Fixpoint list_equiv (L: list node_rep) (omap: option (gmap Z (argmax Z))) : iProp Σ :=
       match L with
       | nil => True
       | pred :: succs => 
         match succs with
-        | nil => ∃ (γ: gname) (h: Z) (t: loc), 
+        | nil => ∃ (γ: gname) (l: val) (t: loc), 
                  (node_next pred +ₗ lvl) ↦{#1 / 2} #t
                  ∗
                  t ↦□ rep_to_node tail
                  ∗
-                 is_lock γ (node_lock pred) (is_array (node_next pred) h)
+                 (node_locks pred +ₗ lvl) ↦□ l
                  ∗
-                 ⌜ lvl < h ⌝
+                 is_lock γ l (in_lock pred)
 
-        | succ :: _ => ∃ (γ: gname) (h: Z) (s: loc), 
+        | succ :: _ => ∃ (v: val_rep) (γ: gname) (l: val) (s: loc), 
                        (node_next pred +ₗ lvl) ↦{#1 / 2} #s
                        ∗
                        s ↦□ rep_to_node succ
                        ∗
-                       is_lock γ (node_lock pred) (is_array (node_next pred) h)
+                       (node_locks pred +ₗ lvl) ↦□ l
                        ∗
-                       ⌜ lvl < h ⌝
+                       is_lock γ l (in_lock pred)
                        ∗
-                       P succ
+                       is_node succ v
                        ∗
-                       list_equiv succs P
+                       ⌜ is_val omap succ v ⌝
+                       ∗
+                       list_equiv succs (opt_delete omap (node_key succ))
         end
       end. 
     
 
-    Lemma list_equiv_cons (rep: node_rep) (L: list node_rep)
-      (P: node_rep → iProp Σ) :
-      list_equiv (rep :: L) P ⊢ 
-        (list_equiv L P ∗ (list_equiv L P -∗ list_equiv (rep :: L) P)).
+    Lemma list_equiv_cons (pred: node_rep) (L: list node_rep) 
+      (omap: option (gmap Z (argmax Z))) :
+      list_equiv (pred :: L) omap ⊢ 
+        ∃ (succ: node_rep), 
+          ( list_equiv L (opt_delete omap (node_key succ))
+            ∗ 
+            (list_equiv L (opt_delete omap (node_key succ)) -∗ list_equiv (pred :: L) omap)).
     Proof.
-      destruct L as [|n].
+      destruct L as [|succ].
       + iIntros "Hrep". by iFrame.
       + iIntros "Hlist". 
-        iDestruct "Hlist" as (γ h s) "(Hpt & Hs & Hlock & Hh & HP & Hmatch)".
-        iFrame. iIntros "Hlist". iFrame.
-        iExists γ, h, s. iFrame.
+        iDestruct "Hlist" as (v γ l s) "(Hpt & Hs & Hl & Hlock & Hnode & Hval & Hmatch)".
+        iExists succ. iFrame.
+        iIntros "Hlist". iFrame.
+        iExists v, γ, l, s. iFrame.
+    Qed.
+
+    Lemma list_equiv_join (s: loc) (head pred succ: node_rep) (L: list node_rep) 
+      (omap: option (gmap Z (argmax Z))) :
+      Sorted node_lt ([head] ++ L ++ [tail]) →
+      pred = head ∨ In pred L →
+      list_equiv ([head] ++ L) omap ⊢
+        (node_next pred +ₗ lvl) ↦{#1/2} #s
+        ∗ 
+        s ↦□ rep_to_node succ
+        -∗
+          ∃ (L1 L2: list node_rep), 
+            ⌜ [head] ++ L ++ [tail] = L1 ++ [pred; succ] ++ L2 ⌝
+            ∗
+            (node_next pred +ₗ lvl) ↦{#1/2} #s
+            ∗ 
+            list_equiv ([head] ++ L) omap.
+    Proof.
+      iIntros (Hsort Hin) "Hlist (Hnext & #Hs)".
+      remember ([head] ++ L) as L' eqn:HeqL'.
+      rewrite -in_inv in Hin.
+
+      iRevert (head omap L HeqL' Hsort Hin) "Hlist".
+      iInduction L' as [|head' L'] "IHL".
+      { iIntros (head omap L Hfalse); inversion Hfalse. }
+
+      iIntros (head omap L HeqL' Hsort Hin) "Hlist".
+      inversion HeqL'; subst.
+      destruct Hin as [Heq|Hin].
+      + subst.
+        destruct L as [|pred' L].
+        - iDestruct "Hlist" as (γ l t) "(Hnext' & #Ht & Hlocks & #Hlock)".
+          iDestruct (mapsto_agree with "Hnext Hnext'") as %Ht.
+          inversion Ht; subst.
+          iDestruct (mapsto_agree with "Hs Ht") as %->%rep_to_node_inj.
+          iExists nil, nil.
+          iSplit; first done. iFrame.
+          iExists γ, l, t. iFrame "# ∗".
+        - iDestruct "Hlist" as (v γ l s') "(Hnext' & #Hs' & #Hl & #Hlock & Hnode & #Hval & Hmatch)".
+          iDestruct (mapsto_agree with "Hnext Hnext'") as %Hs.
+          inversion Hs; subst.
+          iDestruct (mapsto_agree with "Hs Hs'") as %->%rep_to_node_inj.
+          iExists nil, (L ++ [tail]).
+          iSplit; first done. iFrame.
+          iExists v, γ, l, s'. iFrame "# ∗".
+      + destruct L as [|pred' L]; first inversion Hin.
+        iPoseProof ("IHL" with "Hnext") as "IHL'".
+        iPoseProof (list_equiv_cons with "Hlist") as "Hlist".
+        iDestruct "Hlist" as (succ') "(Hlist & Himp)".
+        iPoseProof ("IHL'" $! pred' with "[%] [%] [%] [$]") as (L1 L2) "(%Heq & Hnext & Hlist)".
+        { done. }
+        { 
+          apply node_rep_sorted_app in Hsort as [_ Hsort].
+          rewrite -app_ass //.
+        }
+        { done. }
+
+        iPoseProof ("Himp" with "Hlist") as "Hlist".
+        iExists (head :: L1), L2. iFrame.
+        iPureIntro; simpl in *.
+        rewrite Heq //.
     Qed.
 
     Lemma list_equiv_split (pred succ: node_rep) (L L1 L2: list node_rep) 
-      (P: node_rep → iProp Σ) :
+      (omap: option (gmap Z (argmax Z))) :
       L ++ [tail] = L1 ++ [pred; succ] ++ L2 →
-      list_equiv L P ⊢ 
+      list_equiv L omap ⊢ 
         ∃ (s: loc),
           (node_next pred +ₗ lvl) ↦{#1 / 2} #s
           ∗
           s ↦□ rep_to_node succ
           ∗
-          ((node_next pred +ₗ lvl) ↦{#1 / 2} #s -∗ list_equiv L P).
+          ((node_next pred +ₗ lvl) ↦{#1 / 2} #s -∗ list_equiv L omap).
     Proof.
-      revert L. induction L1 => L HL.
+      revert L omap. induction L1 => L omap HL.
       + destruct L as [|curr L].
         { exfalso. inversion HL. }
         inversion HL as [[H0 HL']]; subst.
         destruct L as [|curr L].
         - inversion HL'; subst.
           iIntros "Hlist".
-          iDestruct "Hlist" as (γ h t) "(Hpt & #Ht & #Hlock & Hh)".
+          iDestruct "Hlist" as (γ l t) "(Hpt & #Ht & #Hl & #Hlock)".
           iExists t. iFrame "# ∗".
           iIntros "Hpt". 
-          iExists γ, h, t. iFrame "# ∗".
+          iExists γ, l, t. iFrame "# ∗".
         - inversion HL'; subst.
           iIntros "Hlist". 
-          iDestruct "Hlist" as (γ h s) "(Hpt & #Hs & #Hlock & Hh & Hmatch)".
+          iDestruct "Hlist" as (v γ l s) "(Hpt & #Hs & #Hl & #Hlock & Hnode & #Hval & Hmatch)".
           iExists s. iFrame "# ∗".
           iIntros "Hpt". 
-          iExists γ, h, s. iFrame "# ∗".
+          iExists v, γ, l, s. iFrame "# ∗".
       + destruct L as [|curr L].
         { 
           exfalso. inversion HL  as [[H0 HL']]; subst. 
@@ -106,7 +245,8 @@ Module ListEquiv (Params: SKIP_LIST_PARAMS).
         }
         
         iIntros "Hlist".
-        iPoseProof (list_equiv_cons with "Hlist") as "(Hlist & Himp)".
+        iPoseProof (list_equiv_cons with "Hlist") as "Hlist".
+        iDestruct "Hlist" as (?) "(Hlist & Himp)".
         iPoseProof (IHL1 with "Hlist") as "Hlist"; auto.
         iDestruct "Hlist" as (s) "(Hpt & #Hs & Himp')".
         iExists s. iFrame "# ∗".
@@ -115,100 +255,147 @@ Module ListEquiv (Params: SKIP_LIST_PARAMS).
     Qed.
 
     Lemma list_equiv_invert_L (L: list node_rep) (head pred: node_rep) 
-      (P: node_rep → iProp Σ) :
+      (omap: option (gmap Z (argmax Z))) :
       In pred L →
-      list_equiv ([head] ++ L) P ⊢ 
-        ∃ (γ: gname) (h: Z) (s: loc) (succ: node_rep), 
+      list_equiv ([head] ++ L) omap ⊢ 
+        ∃ (v: val_rep) (γ: gname) (l: val) (s: loc) (succ: node_rep), 
           (⌜ In succ L ⌝ ∨ ⌜ succ = tail ⌝)
           ∗
           (node_next pred +ₗ lvl) ↦{#1/2} #s
           ∗
           s ↦□ rep_to_node succ
-          ∗ 
-          is_lock γ (node_lock pred) (is_array (node_next pred) h)
           ∗
-          ⌜ lvl < h ⌝
+          (node_locks pred +ₗ lvl) ↦□ l
           ∗
-          P pred
+          is_lock γ l (in_lock pred)
           ∗
-          ((node_next pred +ₗ lvl) ↦{#1/2} #s 
-            ∗ 
-            P pred 
+          is_node pred v
+          ∗
+          ⌜ is_val omap pred v ⌝
+          ∗
+          ∀ (S: gset Z) (v': val_rep),
+            (node_next pred +ₗ lvl) ↦{#1/2} #s 
+            ∗
+            is_node pred v'
+            ∗
+            ⌜ val_v v' ∈ S ⌝
             -∗ 
-              list_equiv ([head] ++ L) P).
+              list_equiv ([head] ++ L) (opt_insert omap (node_key pred) (prodZ S (val_ts v'))).
     Proof.
       iIntros (Hin) "Hlist".
-      iRevert (head Hin) "Hlist".
-      iInduction L as [|succ L] "IHL"; iIntros (head) "Hin"; first by iExFalso.
+      iRevert (head omap Hin) "Hlist".
+      iInduction L as [|succ L] "IHL"; iIntros (head omap) "Hin"; first by iExFalso.
       iDestruct "Hin" as "[%Heq|Hin]"; subst; iIntros "Hlist".
-      + iDestruct "Hlist" as (γ h s) "(Hpt & #Hs & #Hlock & Hh & HP & Hlist)".
+      + iDestruct "Hlist" as (v γ l s) "(Hpt & #Hs & #Hl & #Hlock & Hnode & Hval & Hlist)".
         destruct L as [|next L]; subst.
-        - iDestruct "Hlist" as (γ' h' t) "(Hpt' & #Ht & #Hlock' & #Hh')".
-          iExists γ', h', t, tail. iFrame "# ∗".
-          iSplit; first by iRight.
-          iIntros "(Hpt' & HP)". 
-          iExists γ, h, s. iFrame "# ∗".
-          iExists γ', h', t. iFrame "# ∗".
-        - iDestruct "Hlist" as (γ' h' n) "(Hpt' & #Hn & #Hlock' & #Hh' & Hmatch)".
-          iExists γ', h', n, next. iFrame "# ∗".
-          iSplit; first by iLeft; iRight; iLeft.
-          iIntros "(Hpt' & HP)". 
-          iExists γ, h, s. iFrame "# ∗".
-          iExists γ', h', n. iFrame "# ∗".
-      + iPoseProof (list_equiv_cons with "Hlist") as "(Hlist & Himp)".
-        iPoseProof ("IHL" with "Hin") as "Himp'".
-        iPoseProof ("Himp'" with "Hlist") as "Hlist".
-        iDestruct "Hlist" as (γ h n next) "(%Hnext & Hpt & #Hn & #Hlock & #Hh & HP & Himp')".
-        iExists γ, h, n, next. iFrame "# ∗".
+        - iDestruct "Hlist" as (γ' l' t) "(Hpt' & #Ht & #Hl' & #Hlock')".
+          iExists v, γ', l', t, tail.
+          iFrame "# ∗". iSplit; first by iRight.
+
+          iIntros (S v') "(Hpt' & Hnode & %Hval)". 
+          iExists v', γ, l, s. iFrame "# ∗".
+          iSplit.
+          {
+            destruct omap as [Smap|]; last done.
+            iExists S; rewrite lookup_insert //.
+          }
+          iExists γ', l', t. iFrame "# ∗".
+        - iDestruct "Hlist" as (v' γ' l' n) "(Hpt' & #Hn & #Hl' & #Hlock' & Hnode' & Hval' & Hmatch)".
+          iExists v, γ', l', n, next.
+          iFrame "# ∗". iSplit; first by iLeft; iRight; iLeft.
+          
+          iIntros (S v'') "(Hpt' & Hnode & %Hval)". 
+          iExists v'', γ, l, s. iFrame "# ∗".
+
+          destruct omap as [Smap|].
+          * iSplit.
+            { iExists S; rewrite lookup_insert //. }
+            iExists v', γ', l', n. rewrite /= delete_insert_delete. iFrame "# ∗".
+          * iSplit; first done.
+            iExists v', γ', l', n. iFrame "# ∗".
+      + iDestruct "Hlist" as (v γ l s) "(Hnext & #Hs & #Hl & #Hlock & Hnode & %Hval & Hlist)".
+        iPoseProof ("IHL" with "Hin Hlist") as "Hlist".
+
+        iDestruct "Hlist" as (v' γ' l' s' succ') "(%Hsucc' & Hnext' & #Hs' & #Hl' & #Hlock' & Hnode' & %Hval' & Himp)".
+        iExists v', γ', l', s', succ'. iFrame "# ∗".
         iSplit.
-        { iPureIntro; destruct Hnext; first left; by right. }
-        iIntros "(Hpt & HP)". 
-        iApply "Himp". iApply "Himp'". iFrame.
+        { iPureIntro; destruct Hsucc'; first left; by right. }
+        iSplit.
+        {
+          iPureIntro. 
+          destruct omap as [Smap|]; last done.
+          simpl in *.
+          destruct Hval as [vs [Hsome Hin]]; destruct Hval' as [vs' [Hsome' Hin']].
+          exists vs'. split; last done.
+          rewrite lookup_delete_Some in Hsome'.
+          by destruct Hsome' as [_ Hsome'].
+        }
+
+        iIntros (S v'') "(Hpt'' & Hnode'' & %Hval'')".
+        iPoseProof ("Himp" $! S v'' with "[Hpt'' Hnode'']") as "Hlist".
+        { by iFrame. }
+        iExists v, γ, l, s. 
+        destruct omap as [Smap|]; last iFrame "# ∗".
+        destruct Hval as [vs [Hsome Hin]].
+        destruct Hval' as [vs' [Hsome' Hin']].
+        rewrite lookup_delete_Some in Hsome'.
+        destruct Hsome' as [Hne Hsome'].
+        rewrite /= delete_insert_ne // lookup_insert_ne //.
+        iFrame "# ∗". by iExists vs.
     Qed.
 
     Lemma list_equiv_invert (L: list node_rep) (head pred: node_rep) 
-      (P: node_rep → iProp Σ) :
+      (omap: option (gmap Z (argmax Z))) :
       pred = head ∨ In pred L →
-      list_equiv ([head] ++ L) P ⊢ 
-        ∃ (γ: gname) (h: Z) (s: loc) (succ: node_rep),
+      list_equiv ([head] ++ L) omap ⊢ 
+        ∃ (γ: gname) (l: val) (s: loc) (succ: node_rep),
           (⌜ In succ L ⌝ ∨ ⌜ succ = tail ⌝)
           ∗
           (node_next pred +ₗ lvl) ↦{#1/2} #s
           ∗
           s ↦□ rep_to_node succ
-          ∗ 
-          is_lock γ (node_lock pred) (is_array (node_next pred) h)
           ∗
-          ⌜ lvl < h ⌝
+          (node_locks pred +ₗ lvl) ↦□ l
           ∗
-          ((node_next pred +ₗ lvl) ↦{#1/2} #s -∗ list_equiv ([head] ++ L) P).
+          is_lock γ l (in_lock pred)
+          ∗
+          ((node_next pred +ₗ lvl) ↦{#1/2} #s -∗ list_equiv ([head] ++ L) omap).
     Proof.
       intros Hin; destruct Hin as [Heq|Hin]; first subst.
       + iIntros "Hlist". destruct L as [|next L].
-        - iDestruct "Hlist" as (γ h t) "(Hpt & #Ht & #Hlock & #Hh)".
-          iExists γ, h, t, tail. iFrame "# ∗".
+        - iDestruct "Hlist" as (γ l t) "(Hpt & #Ht & #Hl & #Hlock)".
+          iExists γ, l, t, tail. iFrame "# ∗".
           iSplit; first by iRight.
           iIntros "Hpt". 
-          iExists γ, h, t. iFrame "# ∗".
-        - iDestruct "Hlist" as (γ h n) "(Hpt & #Hn & #Hlock & #Hh & ?)".
-          iExists γ, h, n, next. iFrame "# ∗".
+          iExists γ, l, t. iFrame "# ∗".
+        - iDestruct "Hlist" as (v γ l n) "(Hpt & #Hn & #Hl & #Hlock & ?)".
+          iExists γ, l, n, next. iFrame "# ∗".
           iSplit; first by repeat iLeft.
           iIntros "Hpt". 
-          iExists γ, h, n. iFrame "# ∗".
+          iExists v, γ, l, n. iFrame "# ∗".
       + iIntros "Hlist".
         iPoseProof (list_equiv_invert_L with "Hlist") as "Hlist"; first done.
-        iDestruct "Hlist" as (γ h s succ) "(? & ? & ? & ? & ? & ? & Himp)".
-        iExists γ, h, s, succ. iFrame.
-        iIntros "?". iApply "Himp". iFrame.
+        iDestruct "Hlist" as (? γ l s succ) "(? & ? & ? & ? & ? & Hnode & %Hval & Himp)".
+        iExists γ, l, s, succ. iFrame.
+        iIntros "Hnext". 
+
+        destruct omap as [Smap|].
+        - destruct Hval as [vs [Hsome Hvs]].
+          iPoseProof ("Himp" $! vs v with "[Hnext Hnode]") as "Hlist".
+          { by iFrame. }
+          rewrite /opt_insert insert_id //.
+        - iApply ("Himp" $! {[ val_v v ]} v). iFrame. 
+          rewrite elem_of_singleton //.
     Qed.
 
-    Lemma list_equiv_insert (s n: loc) (head pred new succ: node_rep) 
-      (L: list node_rep) (γ': gname) (h': Z) (P: node_rep → iProp Σ) :
+    Lemma list_equiv_insert (s n: loc) (head pred new succ: node_rep) (L: list node_rep) 
+      (v': val_rep) (γ': gname) (l': val) (omap: option (gmap Z (argmax Z))) :
       node_key new < node_key tail →
       node_key pred < node_key new < node_key succ →
       Sorted node_lt ([head] ++ L ++ [tail]) →
       pred = head ∨ In pred L →
-      list_equiv ([head] ++ L) P ⊢ 
+      opt_lookup omap (node_key new) = None →
+      list_equiv ([head] ++ L) omap ⊢ 
         s ↦□ rep_to_node succ
         ∗ 
         (node_next pred +ₗ lvl) ↦{#1/2} #s
@@ -216,61 +403,68 @@ Module ListEquiv (Params: SKIP_LIST_PARAMS).
         (node_next new +ₗ lvl) ↦{#1/2} #s
         ∗
         n ↦□ rep_to_node new
-        ∗ 
-        is_lock γ' (node_lock new) (is_array (node_next new) h')
         ∗
-        ⌜ lvl < h' ⌝
+        (node_locks new +ₗ lvl) ↦□ l'
         ∗
-        P new
+        is_lock γ' l' (in_lock new)
+        ∗
+        is_node new v'
         -∗ 
-          ∃ (L' L1 L2: list node_rep), 
+          ∃ (L': list node_rep), 
             (node_next pred +ₗ lvl) ↦ #s
-            ∗
-            ⌜ [head] ++ L ++ [tail] = L1 ++ [pred; succ] ++ L2 ⌝
             ∗
             ⌜ Sorted node_lt ([head] ++ L' ++ [tail]) ⌝
             ∗
             ⌜ Permutation ([head] ++ L') ([head; new] ++ L) ⌝ 
             ∗
-            ((node_next pred +ₗ lvl) ↦{#1/2} #n -∗ list_equiv ([head] ++ L') P).
+            ((node_next pred +ₗ lvl) ↦{#1/2} #n 
+              -∗ 
+                list_equiv ([head] ++ L') (opt_insert omap (node_key new) (prodZ {[val_v v']} (val_ts v')))).
     Proof.
-      iIntros (Hnew Hrange Hsort Hin) .
-      iIntros "Hlist (Hs & Hpt & Hpt' & Hn & Hlock' & Hh' & HP')".
+      iIntros (Hnew Hrange Hsort Hin Hnone).
+      iIntros "Hlist (Hs & Hpt & Hpt' & Hn & Hl' & Hlock' & Hnode')".
       remember ([head] ++ L) as L' eqn:HeqL'.
       rewrite -in_inv in Hin.
 
-      iRevert (head L HeqL' Hsort Hin) "Hlist Hs Hpt Hpt' Hn Hlock' Hh' HP'".
+      iRevert (head L omap HeqL' Hsort Hin Hnone) "Hlist Hs Hpt Hpt' Hn Hl' Hlock' Hnode'".
       iInduction L' as [|pred'] "IHL'".
-      { iIntros (head L Hfalse); inversion Hfalse. }
+      { iIntros (head L omap Hfalse); inversion Hfalse. }
 
-      iIntros (head L HeqL' Hsort).
+      iIntros (head L omap HeqL' Hsort).
       inversion HeqL'; subst.
-      iIntros (Hin); inversion Hin as [Heq|HinL].
+      iIntros (Hin Hnone); inversion Hin as [Heq|HinL].
       + subst.
-        iIntros "Hlist #Hs Hpt Hpt' #Hn #Hlock' Hh' HP'".
+        iIntros "Hlist #Hs Hpt Hpt' #Hn #Hl' #Hlock' Hnode'".
         destruct L as [|succ' L].
-        - iDestruct "Hlist" as (γ h t) "(Hpt'' & #Ht & #Hlock & Hh)".
+        - iDestruct "Hlist" as (γ l t) "(Hpt'' & #Ht & #Hl & #Hlock)".
           iDestruct (mapsto_agree with "Hpt Hpt''") as %Heq.
           assert (s = t) as -> by congruence.
           iDestruct (mapsto_agree with "Hs Ht") as %->%rep_to_node_inj.
           
-          iExists (new :: nil), nil, nil.
-          iFrame. iSplit; first done. iSplit.
+          iExists (new :: nil).
+          iFrame. iSplit.
           { 
             iPureIntro; apply Sorted_cons; econstructor; auto.
             all: unfold node_lt; lia.
           }
           iSplit; first auto.
           iIntros "Hpt". 
-          iExists γ, h, n. iFrame "# ∗".
-          iExists γ', h', t. iFrame "# ∗".
-        - iDestruct "Hlist" as (γ h s') "(Hpt'' & #Hs' & #Hlock & Hh & Hmatch)".
+          iExists v', γ, l, n. iFrame "# ∗".
+          iSplit.
+          {
+            destruct omap as [Smap|]; last done.
+            iPureIntro; exists {[val_v v']}.
+            split; last rewrite elem_of_singleton //.
+            rewrite lookup_insert //.
+          }
+          iExists γ', l', t. iFrame "# ∗".
+        - iDestruct "Hlist" as (v γ l s') "(Hpt'' & #Hs' & #Hl & #Hlock & Hnode & #Hval & Hmatch)".
           iDestruct (mapsto_agree with "Hpt Hpt''") as %Heq.
           assert (s = s') as <- by congruence.
           iDestruct (mapsto_agree with "Hs Hs'") as %<-%rep_to_node_inj.
 
-          iExists (new :: succ :: L), nil, (L ++ [tail]).
-          iFrame. iSplit; first done. iSplit.
+          iExists (new :: succ :: L).
+          iFrame. iSplit.
           { 
             iPureIntro.
             repeat apply Sorted_inv in Hsort as (Hsort&?).
@@ -279,23 +473,34 @@ Module ListEquiv (Params: SKIP_LIST_PARAMS).
           }
           iSplit; first auto.
           iIntros "Hpt". 
-          iExists γ, h, n. iFrame "# ∗".
-          iExists γ', h', s. iFrame "# ∗".
+          iExists v', γ, l, n. iFrame "# ∗".
+          iSplit.
+          {
+            destruct omap as [Smap|]; last done.
+            iPureIntro; exists {[val_v v']}.
+            split; last rewrite elem_of_singleton //.
+            rewrite lookup_insert //.
+          }
+          iExists v, γ', l', s.
+          destruct omap as [Smap|]; last iFrame "# ∗".
+          rewrite /= delete_insert; last done.
+          iFrame "# ∗".
       + destruct L as [|next L]; first by inversion HinL.
-        iIntros "Hlist #Hs Hpt Hpt' #Hn #Hlock' Hh' HP'".
+        iIntros "Hlist #Hs Hpt Hpt' #Hn #Hl' #Hlock' Hnode'".
 
         simpl in Hsort; apply Sorted_inv in Hsort as (Hsort&Hhd).
-        iDestruct "Hlist" as (γ h x) "(Hpt'' & #Hx & Hlock & Hh & HP & Hmatch)".
-        iPoseProof ("IHL'" $! next L with "[%] [%] [%] [$] [$] [$] [$] [$] [$] [$] [$]") 
+        iDestruct "Hlist" as (v γ l x) "(Hpt'' & #Hx & #Hl & #Hlock & Hnode & %Hval & Hmatch)".
+        iPoseProof ("IHL'" $! next L with "[%] [%] [%] [%] [$] [$] [$] [$] [$] [$] [$] [$]") 
           as "Hclose"; auto.
-        
-        iDestruct "Hclose" as (L' L1 L2) "(Hpt' & %Hsplit & %Hsort' & %Hperm' & Himp')".
-        iExists (next :: L'), (head :: L1), L2. iFrame.
-        iSplit.
-        {
-          rewrite /= in Hsplit.
-          rewrite /= Hsplit //.
+        { 
+          destruct omap as [Smap|]; last done.
+          simpl in *; destruct Hval as [S [Hsome Hval]].
+          rewrite lookup_delete_ne //.
+          apply (lookup_ne Smap); rewrite Hsome Hnone //.
         }
+        
+        iDestruct "Hclose" as (L') "(Hpt' & %Hsort' & %Hperm' & Himp')".
+        iExists (next :: L'). iFrame.
         iSplit.
         {
           iPureIntro. inversion Hhd.
@@ -309,9 +514,17 @@ Module ListEquiv (Params: SKIP_LIST_PARAMS).
           econstructor; econstructor.
         }
 
-        iIntros "Hpt". iExists γ, h, x.
+        iIntros "Hpt". iExists v, γ, l, x.
         iPoseProof ("Himp'" with "Hpt") as "Hlist".
-        iFrame "# ∗".
+        destruct omap as [Smap|]; last iFrame "# ∗".
+        simpl in *; destruct Hval as [S [Hsome Hval]].
+        assert (node_key next ≠ node_key new) as Hne.
+        { apply (lookup_ne Smap); rewrite Hsome Hnone //. }
+
+        rewrite delete_insert_ne; last first. 
+        { apply (lookup_ne Smap); rewrite Hsome Hnone //. }
+        iFrame "# ∗"; iPureIntro.
+        exists S. rewrite lookup_insert_ne //.
     Qed.
 
   End Proofs.
