lib/node_rep.v
@@ -1,33 +1,36 @@
 From iris.heap_lang Require Import notation.
 
+
 Local Open Scope Z.
 
 Definition val_rep : Type := Z * Z * loc.
 
 Definition val_v (v: val_rep) : Z := v.1.1.
 Definition val_ts (v: val_rep) : Z := v.1.2.
-Definition val_next (v: val_rep) : loc := v.2.
+Definition val_prev (v: val_rep) : loc := v.2.
 
 Definition valV : val := λ: "l", Fst (Fst "l").
 Definition valTs : val := λ: "l", Snd (Fst "l").
-Definition valNext : val := λ: "l", Snd "l".
+Definition valPrev : val := λ: "l", Snd "l".
 
 Definition rep_to_val (v: val_rep) : val := 
-  (#(val_v v), #(val_ts v), #(val_next v)).
+  (#(val_v v), #(val_ts v), #(val_prev v)).
 
-Definition node_rep : Type := Z * loc * loc * option loc * val.
+Definition node_rep : Type := Z * loc * loc * option loc * val * loc.
 
-Definition node_key (n: node_rep) : Z := n.1.1.1.1.
-Definition node_val (n: node_rep) : loc := n.1.1.1.2.
-Definition node_next (n: node_rep) : loc := n.1.1.2.
-Definition node_down (n: node_rep) : option loc := n.1.2.
-Definition node_lock (n: node_rep) : val := n.2.
+Definition node_key (n: node_rep) : Z := n.1.1.1.1.1.
+Definition node_val (n: node_rep) : loc := n.1.1.1.1.2.
+Definition node_next (n: node_rep) : loc := n.1.1.1.2.
+Definition node_down (n: node_rep) : option loc := n.1.1.2.
+Definition node_lock (n: node_rep) : val := n.1.2.
+Definition node_locks (n: node_rep) : loc := n.2.
 
-Definition nodeKey : val := λ: "l", Fst (Fst (Fst (Fst "l"))).
-Definition nodeVal : val := λ: "l", Snd (Fst (Fst (Fst "l"))).
-Definition nodeNext : val := λ: "l", Snd (Fst (Fst "l")).
-Definition nodeDown : val := λ: "l", Snd (Fst "l").
-Definition nodeLock : val := λ: "l", Snd "l".
+Definition nodeKey : val := λ: "l", Fst (Fst (Fst (Fst (Fst "l")))).
+Definition nodeVal : val := λ: "l", Snd (Fst (Fst (Fst (Fst "l")))).
+Definition nodeNext : val := λ: "l", Snd (Fst (Fst (Fst "l"))).
+Definition nodeDown : val := λ: "l", Snd (Fst (Fst "l")).
+Definition nodeLock : val := λ: "l", Snd (Fst "l").
+Definition nodeLocks : val := λ: "l", Snd "l".
 
 Definition oloc_to_val (ol: option loc) : val := 
   match ol with
@@ -36,19 +39,20 @@ Definition oloc_to_val (ol: option loc) : val :=
   end.
 
 Definition rep_to_node (n: node_rep) : val :=
-  (#(node_key n), #(node_val n), #(node_next n), oloc_to_val (node_down n), (node_lock n)).
+  (#(node_key n), #(node_val n), #(node_next n), oloc_to_val (node_down n), (node_lock n), #(node_locks n)).
 
 Definition dummy_null : loc := {|loc_car := 0|}.
 Definition dummy_lock : val := #().
+Definition dummy_val : val_rep := (0, 0, dummy_null).
 
 
 Lemma fold_rep_to_val (v: val_rep) :
-  ((#(val_v v), #(val_ts v), #(val_next v)))%V =
+  ((#(val_v v), #(val_ts v), #(val_prev v)))%V =
   rep_to_val v.
 Proof. done. Qed.
 
 Lemma fold_rep_to_node (n: node_rep) :
-  ((#(node_key n), #(node_val n), #(node_next n), oloc_to_val (node_down n), (node_lock n)))%V =
+  ((#(node_key n), #(node_val n), #(node_next n), oloc_to_val (node_down n), (node_lock n), #(node_locks n)))%V =
   rep_to_node n.
 Proof. done. Qed.
 
@@ -58,7 +62,7 @@ Lemma rep_to_val_inj rep rep' :
 Proof.
   destruct rep as ((?&?)&?).
   destruct rep' as ((?&?)&?).
-  rewrite /rep_to_val/val_v/val_ts/val_next/=.
+  rewrite /rep_to_val/val_v/val_ts/val_prev/=.
   intros; congruence.
 Qed.
 
@@ -66,9 +70,9 @@ Lemma rep_to_node_inj rep rep':
   rep_to_node rep = rep_to_node rep' →
   rep = rep'.
 Proof.
-  destruct rep as ((((?&v)&?)&down)&?). 
-  destruct rep' as ((((?&v')&?)&down')&?).
-  rewrite /rep_to_node/node_key/node_val/node_next/node_down/node_lock//=.
+  destruct rep as (((((?&v)&?)&down)&?)&?). 
+  destruct rep' as (((((?&v')&?)&down')&?)&?).
+  rewrite /rep_to_node/node_key/node_val/node_next/node_down/node_lock/node_locks//=.
   destruct down; destruct down'.
   all: inversion 1; congruence.
 Qed.
