jellyfish/spec/insert.v
@@ -1,0 +1,342 @@
+From iris.base_logic.lib Require Import invariants.
+From iris.algebra Require Import auth frac_auth gset gmap.
+From iris.heap_lang Require Import proofmode.
+
+From SkipList.lib Require Import arg_max.
+From SkipList.jellyfish Require Import code.
+From SkipList.lib Require Import misc node_rep node_lt key_equiv.
+From SkipList.jellyfish.inv Require Import list_equiv lazy_inv skip_inv.
+From SkipList.jellyfish.spec Require Import link.
+
+
+Local Open Scope Z.
+
+Module InsertSpec (Params: SKIP_LIST_PARAMS).
+  Import Params.
+  Module Link := LinkSpec Params.
+  Export Link.
+
+  Section Proofs.
+    Context `{!heapGS Σ, !gset_list_unionGS Σ, !lockG Σ}.
+
+    Theorem update_spec (v ts: Z) (head curr: node_rep) 
+      (Smap: gmap Z (argmax Z)) (q: frac)
+      (sub: sub_gname) (bot: bot_gname) 
+      (val: val_rep) :
+      {{{
+        is_bot_list 0 head Smap q bot sub
+        ∗
+        own (s_auth sub) (◯ {[ curr ]})
+        ∗
+        (node_val curr) ↦{#1 / 2} rep_to_val val
+      }}}
+        update (rep_to_node curr) #v #ts
+      {{{ val', RET #();
+        is_bot_list 0 head (Smap ⋅ {[ node_key curr := prodZ {[ v ]} ts ]}) q bot sub
+        ∗
+        (node_val curr) ↦{#1 / 2} rep_to_val val'
+        ∗
+        if decide (ts < val_ts val) then ⌜ val = val' ⌝  
+                                    else ⌜ val_v val' = v ⌝
+                                         ∗
+                                         ⌜ val_ts val' = ts ⌝
+                                         ∗
+                                         (val_prev val') ↦□ rep_to_val val
+      }}}.
+    Proof.
+      iIntros (Φ) "((Hown_frag & #Hinv) & #Hown_succ & Hval) HΦ".
+
+      wp_lam. wp_pures. wp_lam. wp_pures.
+      wp_load. wp_let. wp_lam. wp_pures.
+
+      case_bool_decide as Hts; wp_if.
+      + iInv (levelN 0) as (S' Smap' L) "(Hinv_sub & Hinv_bot)" "Hclose".
+        iDestruct "Hinv_sub" as "(>%Hperm & >%Hsort & >%Hequiv & >Hown_auth & >Hown_toks & Hlist)".
+        iDestruct "Hinv_bot" as "(>Hown_frac & >Hown_keys)".
+
+        iAssert ⌜ In curr L ⌝%I with "[Hown_auth]" as %Hin.
+        {
+          iDestruct (own_valid_2 with "Hown_auth Hown_succ") 
+            as %[Hvalid%gset_included]%auth_both_valid_discrete.
+          rewrite -elem_of_list_In Hperm elem_of_elements.
+          iPureIntro; set_solver.
+        }
+
+        rewrite list_equiv_invert_L; last done.
+        iDestruct "Hlist" as (val' γ l s succ) "(_ & Hpt & _ & _ & _ & >Hnode & >%Hval & Himp)".
+        iDestruct (mapsto_agree with "Hval Hnode") as %<-%rep_to_val_inj.
+        destruct Hval as [vs [Hsome Hv]].
+
+        assert (Smap ⋅ ∅ = Smap) as <- by rewrite right_id_L //.
+        rewrite -(Qp_div_2 q) frac_auth_frag_op.
+        iDestruct "Hown_frag" as "(Hown_frag & Hown_emp)".
+        iMod (own_update_2 with "Hown_frac Hown_emp") as "[Hown_frac Hown_emp]".
+        { 
+          apply frac_auth_update. 
+          apply (insert_alloc_local_update _ _ 
+            (node_key curr) 
+            (prodZ vs (val_ts val)) 
+            (prodZ {[v]} ts ⋅ prodZ vs (val_ts val)) 
+            (prodZ {[v]} ts)
+          ); auto.
+          apply arg_max_local_update.
+        }
+
+        rewrite arg_max_lt; last done.
+        rewrite insert_id; last done.
+        rewrite insert_singleton_op; last done.
+        do 2 rewrite right_id_L.
+        iCombine "Hown_frag Hown_emp" as "Hown_frag".
+        rewrite Qp_div_2.
+
+        iPoseProof ("Himp" $! vs val with "[Hpt Hnode]") as "Hlist".
+        { iNext; by iFrame. }
+        rewrite /opt_map /opt_insert insert_id //.
+        iMod ("Hclose" with "[Hlist Hown_auth Hown_toks Hown_frac Hown_keys]") as "_".
+        { iNext; iExists S', Smap', L; by iFrame "# ∗". }
+        iModIntro; iApply ("HΦ" $! val).
+        iFrame "# ∗".
+        by destruct (decide (ts < val_ts val)).
+      + wp_alloc v' as "Hval'"; wp_pures.
+        iInv (levelN 0) as (S' Smap' L) "(Hinv_sub & Hinv_bot)" "Hclose".
+        iDestruct "Hinv_sub" as "(>%Hperm & >%Hsort & >%Hequiv & >Hown_auth & >Hown_toks & Hlist)".
+        iDestruct "Hinv_bot" as "(>Hown_frac & >Hown_keys)".
+
+        iAssert ⌜ In curr L ⌝%I with "[Hown_auth]" as %Hin.
+        {
+          iDestruct (own_valid_2 with "Hown_auth Hown_succ") 
+            as %[Hvalid%gset_included]%auth_both_valid_discrete.
+          rewrite -elem_of_list_In Hperm elem_of_elements.
+          iPureIntro; set_solver.
+        }
+
+        rewrite list_equiv_invert_L; last done.
+        iDestruct "Hlist" as (val' γ l s succ) "(_ & Hpt & _ & _ & _ & >Hnode & >%Hval & Himp)".
+        iDestruct (mapsto_agree with "Hval Hnode") as %<-%rep_to_val_inj.
+        destruct Hval as [vs [Hsome Hv]].
+
+        assert (Smap ⋅ ∅ = Smap) as <- by rewrite right_id_L //.
+        rewrite -(Qp_div_2 q) frac_auth_frag_op.
+        iDestruct "Hown_frag" as "(Hown_frag & Hown_emp)".
+        iMod (own_update_2 with "Hown_frac Hown_emp") as "[Hown_frac Hown_emp]".
+        { 
+          apply frac_auth_update. 
+          apply (insert_alloc_local_update _ _ 
+            (node_key curr) 
+            (prodZ vs (val_ts val)) 
+            (prodZ {[v]} ts ⋅ prodZ vs (val_ts val)) 
+            (prodZ {[v]} ts)
+          ); auto.
+          apply arg_max_local_update.
+        }
+
+        rewrite (insert_singleton_op _ _ (prodZ {[v]} ts)); last done.
+        do 2 rewrite right_id_L.
+        iCombine "Hown_frag Hown_emp" as "Hown_frag".
+        rewrite Qp_div_2.
+
+        set (val' := (v, ts, v')).
+        rewrite (fold_rep_to_val val').
+        iCombine "Hval Hnode" as "Hval".
+        wp_store.
+        iDestruct "Hval" as "(Hval & Hnode)".
+        iMod (mapsto_persist with "Hval'") as "#Hval'".
+
+        assert (val_ts val = ts ∨ val_ts val < ts) as Hts_range by lia.
+        clear Hts; destruct Hts_range as [->|Hlt].
+        - rewrite arg_max_eq.
+          iPoseProof ("Himp" $! ({[ v ]} ∪ vs) val' with "[Hpt Hnode]") as "Hlist".
+          { iFrame; iPureIntro; by apply elem_of_union_l, elem_of_singleton. }
+
+          assert (dom (<[node_key curr:=prodZ ({[v]} ∪ vs) ts]> Smap') = dom Smap') as Hdom.
+          { apply dom_insert_lookup_L; by exists (prodZ vs (val_ts val)). }
+          rewrite -Hdom; rewrite -Hdom in Hequiv.
+
+          iMod ("Hclose" with "[Hlist Hown_auth Hown_toks Hown_frac Hown_keys]") as "_".
+          { iNext; iExists S', (<[node_key curr:=prodZ ({[v]} ∪ vs) ts]> Smap'), L; by iFrame "# ∗". }
+          iModIntro; iApply ("HΦ" $! val').
+          iFrame "# ∗".
+          destruct (decide (ts < ts)); first lia.
+          by iFrame "#".
+        - rewrite arg_max_op arg_max_comm -arg_max_op arg_max_lt; last done.
+          iPoseProof ("Himp" $! {[ v ]} val' with "[Hpt Hnode]") as "Hlist".
+          { iFrame; iPureIntro; by apply elem_of_singleton. }
+
+          assert (dom (<[node_key curr:=prodZ {[v]} ts]> Smap') = dom Smap') as Hdom.
+          { apply dom_insert_lookup_L; by exists (prodZ vs (val_ts val)). }
+          rewrite -Hdom; rewrite -Hdom in Hequiv.
+
+          iMod ("Hclose" with "[Hlist Hown_auth Hown_toks Hown_frac Hown_keys]") as "_".
+          { iNext; iExists S', (<[node_key curr:=prodZ {[v]} ts]> Smap'), L; by iFrame "# ∗". }
+          iModIntro; iApply ("HΦ" $! val').
+          iFrame "# ∗".
+          destruct (decide (ts < val_ts val)); first lia.
+          by iFrame "#".
+    Qed.
+
+    Theorem tryInsert_spec (key v ts h: Z) (head curr: node_rep) 
+      (Smap: gmap Z (argmax Z)) (q: frac)
+      (sub: sub_gname) (bot: bot_gname) :
+      INT_MIN < key < INT_MAX →
+      {{{
+        is_bot_list 0 head Smap q bot sub
+        ∗
+        (⌜ curr = head ⌝ ∨ own (s_auth sub) (◯ {[ curr ]}))
+        ∗
+        ⌜ node_key curr < key ⌝
+        ∗
+        ⌜ 0 ≤ h ⌝ 
+      }}}
+        tryInsert (rep_to_node curr) #key #v #ts #h
+      {{{ (opt: val) (n: loc) (new: node_rep), RET opt;
+        is_bot_list 0 head (Smap ⋅ {[ key := prodZ {[ v ]} ts ]}) q bot sub
+        ∗
+        ( 
+          ⌜ opt = NONEV ⌝ ∨ 
+          ( 
+            ⌜ opt = SOMEV #n ⌝ 
+            ∗ 
+            own (s_auth sub) (◯ {[ new ]})
+            ∗ 
+            own (s_toks sub) (GSet {[ node_key new ]})
+            ∗ 
+            own (s_keys bot) (GSet {[ node_key new ]})
+            ∗ 
+            ⌜ node_key new = key ⌝
+            ∗
+            n ↦□ rep_to_node new
+            ∗
+            (node_next new +ₗ 1) ↦∗ replicate (Z.to_nat h) #()
+            ∗
+            (node_locks new +ₗ 1) ↦∗ replicate (Z.to_nat h) #()
+          )
+        )
+      }}}.
+    Proof.
+      iIntros (Hkey_range Φ) "((Hown_frag & #Hinv) & #Hown_curr & %Hrange & %Hh) HΦ".
+      wp_lam. wp_pures.
+
+      wp_apply findLock_spec.
+      { iFrame "#". iPureIntro; lia. }
+      iIntros (pred succ) "(%Hrange' & #Hown_pred & #Hown_succ & Hlock)".
+      iDestruct "Hlock" as (γ l s) "(#Hl & #Hlock & Hnext & #Hs & Hval & Hlocked)".
+      do 2 rewrite loc_add_0.
+
+      wp_pures. wp_lam. wp_pures. wp_load. 
+      wp_pures. wp_lam. wp_pures.
+      case_bool_decide as Hcase; wp_if.
+      + assert (key = node_key succ) as Heq by congruence.
+        iDestruct "Hown_succ" as "[Hown_succ|%Hsucc]"; last first.
+        { subst; exfalso. rewrite /node_key/tail/= in Hkey_range; lia. }
+        iDestruct "Hval" as "[%Hsucc|Hval]".
+        { subst; exfalso. rewrite /node_key/tail/= in Hkey_range; lia. }
+        iDestruct "Hval" as (val) "Hval".
+
+        wp_apply (update_spec with "[$]").
+        iIntros (val') "((Hown_frag & _) & Hval & _)".
+        wp_pures.
+
+        wp_apply (release_spec with "[Hnext Hval Hlocked]").
+        { 
+          iFrame "# ∗"; iExists s, succ; rewrite loc_add_0; iFrame "# ∗". 
+          iRight; by iExists val'.
+        }
+        iIntros "_". wp_pures.
+        iModIntro; iApply "HΦ".
+        rewrite -Heq. iFrame "# ∗". by iLeft.
+      + assert (key ≠ node_key succ) as Hneq by congruence.
+
+        wp_apply (createAndLink_spec with "[Hnext Hval Hown_frag]").
+        { done. }
+        { iFrame "# ∗". iPureIntro; lia. }
+        iIntros (n new) "((Hown_map & _) & Hown_frag & Hown_tok & Hown_key & Hkey & Hnext & #Hn & Hval & Hnexts & Hlocks)".
+        wp_let.
+
+        wp_apply (release_spec with "[Hnext Hval Hlocked]").
+        { iFrame "# ∗"; iExists n, new; rewrite loc_add_0; iFrame "# ∗". }
+        iIntros "_"; wp_pures.
+        iModIntro; iApply ("HΦ" $! _ n new).
+        iFrame "# ∗". iRight; by iFrame.
+    Qed.
+
+    Theorem insert_spec (lvl: Z) (head curr new: node_rep) 
+      (bot: bot_gname) (top_sub bot_sub: sub_gname) (n: loc) :
+      INT_MIN < node_key new < INT_MAX →
+      {{{
+        inv (levelN lvl) (lazy_list_inv lvl head bot top_sub (Some bot_sub))
+        ∗
+        (⌜ curr = head ⌝ ∨ own (s_auth top_sub) (◯ {[ curr ]}))
+        ∗
+        ⌜ node_key curr < node_key new ⌝
+        ∗ 
+        own (s_auth bot_sub) (◯ {[ new ]})
+        ∗ 
+        own (s_toks bot_sub) (GSet {[ node_key new ]})
+        ∗
+        n ↦□ rep_to_node new
+        ∗
+        (node_next new +ₗ lvl) ↦ #()
+        ∗
+        (node_locks new +ₗ lvl) ↦ #()
+      }}}
+        insert (rep_to_node curr) #lvl #n
+      {{{ RET #();
+        own (s_auth top_sub) (◯ {[ new ]})
+        ∗ 
+        own (s_toks top_sub) (GSet {[ node_key new ]})
+      }}}.
+    Proof.
+      iIntros (Hkey_range Φ) "(#Hinv & #Hown_curr & %Hrange & Hown_frag & Hown_tok & #Hn & Hnext & Hlocks) HΦ".
+      wp_lam. wp_let. wp_let.
+      wp_load. wp_lam. wp_pures.
+
+      wp_apply findLock_spec.
+      { iFrame "#". iPureIntro; lia. }
+      iIntros (pred succ) "(%Hrange' & #Hown_pred & #Hown_succ & Hlock)".
+      iDestruct "Hlock" as (γ l s) "(#Hl & #Hlock & Hnext' & #Hs & Hval & Hlocked)".
+      wp_pures. wp_lam. wp_pures.
+
+      wp_bind (Load _).
+      iInv (levelN lvl) as (S' Smap' L) "(Hinv_sub & _)" "Hclose".
+      iDestruct "Hinv_sub" as "(>%Hperm & >%Hsort & >%Hequiv' & >Hown_auth & >Hown_toks & Hlist)".
+      wp_load.
+
+      iAssert ⌜ node_key new ≠ node_key succ ⌝%I
+        with "[Hown_auth Hown_succ Hown_tok Hlist]" as %Hneq.
+      {
+        iDestruct "Hown_succ" as "[Hown|%Heq]"; last first.
+        { iPureIntro; rewrite Heq /tail/node_key/=; rewrite /node_key in Hkey_range; lia. } 
+
+        iDestruct (own_valid_2 with "Hown_auth Hown") 
+          as %[Hvalid%gset_included]%auth_both_valid_discrete.
+
+        assert (In succ L).
+        { rewrite -elem_of_list_In Hperm elem_of_elements. set_solver. }
+
+        rewrite list_equiv_invert_L; last done.
+        iDestruct "Hlist" as (? ? ? ? ?) "(_ & _ & _ & _ & _ & Hnode & _)".
+        iDestruct "Hnode" as "(_ & Hown_tok')".
+
+        iDestruct (own_valid_2 with "Hown_tok Hown_tok'") as 
+          %Hdisj%gset_disj_valid_op.
+        iPureIntro; set_solver.
+      }
+
+      iMod ("Hclose" with "[Hlist Hown_auth Hown_toks]") as "_".
+      { iNext; iExists S', Smap', L; by iFrame "# ∗". }
+      iModIntro; wp_pures.
+
+      wp_apply (link_spec with "[Hnext' Hown_frag Hown_tok Hnext Hlocks]").
+      { done. }
+      { iFrame "# ∗". iPureIntro; lia. }
+      iIntros "(Hown_frag & Hown_tok & Hnext)".
+
+      wp_pures.
+      wp_apply (release_spec with "[Hnext Hlocked]").
+      { iFrame "# ∗"; iExists n, new; iFrame "# ∗". }
+      iIntros "_"; iApply "HΦ"; iFrame.
+      Unshelve. done.
+    Qed.
+
+  End Proofs.
+End InsertSpec.
