jellyfish/spec/put.v
@@ -1,0 +1,317 @@
+From iris.algebra Require Import auth frac_auth gset gmap.
+From iris.heap_lang Require Import proofmode.
+
+From SkipList.lib Require Import arg_max.
+From SkipList.jellyfish Require Import code.
+From SkipList.lib Require Import misc node_rep node_lt key_equiv.
+From SkipList.jellyfish.inv Require Import list_equiv lazy_inv skip_inv.
+From SkipList.jellyfish.spec Require Import insert.
+
+
+Local Open Scope Z.
+
+Module AddSpec (Params: SKIP_LIST_PARAMS).
+  Import Params.
+  Module Insert := InsertSpec Params.
+  Export Insert.
+
+  Section Proofs.
+    Context `{!heapGS Σ, !gset_list_unionGS Σ, !lockG Σ}.
+
+    Theorem topLevel_spec (key h lvl: Z) (head curr: node_rep) 
+      (Smap: gmap Z (argmax Z)) (q: frac) (bot: bot_gname) 
+      (top_sub: sub_gname) (bot_subs: list sub_gname) :
+      {{{
+        skip_list_equiv lvl head Smap q bot (top_sub :: bot_subs)
+        ∗
+        (⌜ curr = head ⌝ ∨ own (s_auth top_sub) (◯ {[ curr ]}))
+        ∗
+        ⌜ node_key curr < key < INT_MAX ⌝
+        ∗
+        ⌜ 0 ≤ h ≤ lvl ⌝
+      }}}
+        topLevel (rep_to_node curr) #key #h #lvl
+      {{{ curr' top_sub' bot_subs', RET rep_to_node curr';
+        skip_list_equiv h head Smap q bot (top_sub' :: bot_subs')
+        ∗
+        (⌜ curr' = head ⌝ ∨ own (s_auth top_sub') (◯ {[ curr' ]}))
+        ∗
+        ⌜ node_key curr' < key < INT_MAX ⌝
+        ∗
+        ∀ (v ts: Z),
+          skip_list_equiv h head (Smap ⋅ {[ key := prodZ {[ v ]} ts ]}) q bot (top_sub' :: bot_subs')
+          -∗
+          skip_list_equiv lvl head (Smap ⋅ {[ key := prodZ {[ v ]} ts ]}) q bot (top_sub :: bot_subs)
+      }}}.
+    Proof.
+      iIntros (Φ) "(Hlist & Hown_curr & Hcurr_range & Hh) HΦ".
+      iRevert (curr head lvl top_sub bot_subs) "Hlist Hown_curr Hcurr_range Hh HΦ".
+      iLöb as "IH".
+      iIntros (curr head lvl top_sub bot_subs) "Hlist #Hown_curr %Hcurr_range %Hh HΦ".
+
+      wp_lam. wp_let. wp_let. wp_let.
+
+      rewrite skip_list_equiv_cons.
+      iDestruct "Hlist" as (obot) "(Hinv & Hlist)".
+      wp_apply (find_sub_spec with "[Hinv]").
+      { by iFrame "# ∗". }
+
+      iIntros (pred succ) "(%Hrange' & #Hown_pred & #Hown_succ & _)".
+      wp_pures.
+      case_bool_decide as Hcase; wp_if.
+      + inversion Hcase; subst.
+        iModIntro; iApply "HΦ".
+        iFrame "# ∗". 
+        iSplit; first (iPureIntro; lia).
+        iIntros (v ts) "?"; iFrame.
+      + assert (h ≠ lvl) by congruence.
+        destruct bot_subs as [|bot_sub bot_subs].
+        { iDestruct "Hlist" as "(%Hfalse & _)"; lia. }
+        iDestruct "Hlist" as "(#Hlvl & #Hinv & Hmatch)"; unfold is_sub_list.
+
+        wp_bind (BinOp _ _ _).
+        iInv (levelN lvl) as (S' Smap' L) "(Hinv_sub & _)" "Hclose".
+        iDestruct "Hinv_sub" as "(>%Hperm & >%Hsort & >%Hequiv & >Hown_auth & >Hown_toks & Hlist)".
+
+        iDestruct "Hown_pred" as "[%Heq | #Hown_pred]".
+        - wp_op.
+          iMod ("Hclose" with "[Hlist Hown_auth Hown_toks]") as "_".
+          { iNext; iExists S', Smap', L; by iFrame. }
+          iModIntro.
+
+          iApply ("IH" with "Hmatch [] [%] [%]").
+          { by iLeft. }
+          { lia. }
+          { lia. }
+
+          iNext. 
+          iIntros (curr' top_sub' bot_subs').
+          iIntros "(Hlist & Hown_curr' & Hcurr_range' & Himp)".
+          iApply "HΦ". iFrame "# ∗".
+        - iDestruct (own_valid_2 with "Hown_auth Hown_pred") 
+            as %[Hvalid%gset_included]%auth_both_valid_discrete.
+
+          rewrite (list_equiv_invert_L _ _ _ _ pred); last first.
+          { rewrite Hperm -elem_of_list_In elem_of_elements; set_solver. }
+
+          iDestruct "Hlist" as (? ? ? ? ?) "(_ & Hpt & #Hs & _ & _ & Hnode & _ & Himp)".
+          iDestruct "Hnode" as "(Hown_frag & Hown_tok)".
+          assert ({[ pred ]} = {[ pred ]} ⋅ {[ pred ]}) as -> by set_solver.
+          iDestruct "Hown_frag" as "(Hown_frag & Hown_frag_dup)".
+          assert ({[ pred ]} = {[ pred ]} ⋅ {[ pred ]}) as <- by set_solver.
+
+          wp_op.
+          iPoseProof ("Himp" $! {[ val_v dummy_val ]} dummy_val with "[Hpt Hown_frag_dup Hown_tok]") as "Hlist".
+          { iFrame; rewrite elem_of_singleton //. }
+          iMod ("Hclose" with "[Hlist Hown_auth Hown_toks]") as "_".
+          { iNext; iExists S', Smap', L; by iFrame. }
+          iModIntro.
+        
+          iApply ("IH" with "Hmatch [$] [%] [%]").
+          { lia. }
+          { lia. }
+
+          iNext.
+          iIntros (curr' top_sub' bot_subs').
+          iIntros "(Hlist & Hown_curr' & Hcurr_range' & Himp)".
+          iApply "HΦ". iFrame "# ∗".
+    Qed.
+
+    Theorem putAll_spec (key v ts h lvl: Z) (head curr: node_rep) 
+      (Smap: gmap Z (argmax Z)) (q: frac) (bot: bot_gname) 
+      (top_sub: sub_gname) (bot_subs: list sub_gname) :
+      INT_MIN < key < INT_MAX →
+      {{{
+        skip_list_equiv lvl head Smap q bot (top_sub :: bot_subs)
+        ∗
+        (⌜ curr = head ⌝ ∨ own (s_auth top_sub) (◯ {[ curr ]}))
+        ∗
+        ⌜ node_key curr < key ⌝
+        ∗
+        ⌜ 0 ≤ lvl ≤ h ⌝
+      }}}
+        putAll (rep_to_node curr) #key #v #ts #h #lvl
+      {{{ (opt: val) (n: loc) (new: node_rep), RET opt;
+        skip_list_equiv lvl head (Smap ⋅ {[ key := prodZ {[ v ]} ts ]}) q bot (top_sub :: bot_subs)
+        ∗
+        ( 
+          ⌜ opt = NONEV ⌝ ∨ 
+          ( 
+            ⌜ opt = SOMEV #n ⌝ 
+            ∗ 
+            own (s_auth top_sub) (◯ {[ new ]})
+            ∗ 
+            own (s_toks top_sub) (GSet {[ node_key new ]})
+            ∗ 
+            own (s_keys bot) (GSet {[ node_key new ]})
+            ∗ 
+            ⌜ node_key new = key ⌝
+            ∗
+            n ↦□ rep_to_node new
+            ∗
+            (node_next new +ₗ lvl +ₗ 1) ↦∗ replicate (Z.to_nat (h - lvl)) #()
+            ∗
+            (node_locks new +ₗ lvl +ₗ 1) ↦∗ replicate (Z.to_nat (h - lvl)) #()
+          )
+        )
+      }}}.
+    Proof.
+      iIntros (Hkey_range Φ) "(Hlist & Hown_curr & Hrange & Hh) HΦ".
+      iRevert (Φ curr head lvl top_sub bot_subs) "Hlist Hown_curr Hrange Hh HΦ".
+      iLöb as "IH".
+      iIntros (Φ curr head lvl top_sub bot_subs) "Hlist #Hown_curr %Hrange %Hh HΦ".
+
+      wp_lam. wp_pures.
+      iPoseProof (skip_list_equiv_cons with "Hlist") as (obot) "(Hinv & Hlist)".
+      wp_apply (find_sub_spec with "[Hinv]").
+      { iFrame "# ∗". iPureIntro; lia. }
+
+      iIntros (pred succ) "(%Hrange' & #Hown_pred & #Hown_succ & _)".
+      wp_pures. 
+
+      destruct bot_subs as [|bot_sub bot_subs].
+      + iDestruct "Hlist" as "(%Hlvl & (Hown_frag & #Hinv))".
+        rewrite Hlvl; wp_pures.
+
+        wp_apply (tryInsert_spec with "[Hown_frag]").
+        { done. }
+        { iFrame "# ∗". iPureIntro; lia. }
+        iIntros (opt n new) "((Hown_frac & _) & Hopt)".
+
+        iApply "HΦ". 
+        do 2 rewrite loc_add_0.
+        assert (h - 0 = h) as -> by lia.
+        by iFrame "# ∗".
+      + iDestruct "Hlist" as "(%Hlvl & #Hinv & Hmatch)"; unfold is_sub_list.
+        case_bool_decide as Hcase; wp_if.
+        - exfalso; inversion Hcase; lia.
+        - wp_bind (BinOp _ _ _).
+          iInv (levelN lvl) as (S' Smap' L) "(Hinv_sub & _)" "Hclose".
+          iDestruct "Hinv_sub" as "(>%Hperm & >%Hsort & >%Hequiv & >Hown_auth & >Hown_toks & Hlist)".
+      
+          iDestruct "Hown_pred" as "[%Heq | #Hown_pred]".
+          * wp_op.
+            iMod ("Hclose" with "[Hlist Hown_auth Hown_toks]") as "_".
+            { iNext; iExists S', Smap', L; by iFrame. }
+            iModIntro. 
+
+            wp_bind (putAll _ _ _ _ _ _).
+            iApply ("IH" with "Hmatch [] [%] [%]").
+            { by iLeft. }
+            { lia. }
+            { lia. }
+
+            iNext; iIntros (opt n new) "(Hlist & Hopt)".
+            iDestruct "Hopt" as "[%Hopt | (%Hopt & Hown_frag & Hown_tok & Hown_key & %Hkey & #Hn & Hnext & Hlocks)]".
+            ++ rewrite Hopt; wp_pures.
+               iModIntro; iApply ("HΦ" $! _ n new).
+               iSplitR ""; last by iLeft.
+               by iFrame "# ∗".
+            ++ rewrite Hopt. wp_pures.
+
+               do 2 rewrite loc_add_assoc.
+               assert (Z.to_nat (h - (lvl - 1)) = S (Z.to_nat (h - lvl)))%nat as -> by lia.
+               assert (lvl - 1 + 1 = lvl) as -> by lia.
+               rewrite replicate_S ?array_cons.
+               iDestruct "Hnext" as "(Hnext' & Hnext)".
+               iDestruct "Hlocks" as "(Hlocks' & Hlocks)".
+
+               wp_apply (insert_spec _ _ _ new with "[Hown_frag Hown_tok Hnext' Hlocks']").
+               { rewrite Hkey //. }
+               { 
+                 iFrame "# ∗".
+                 iSplit; first by iLeft.
+                 iPureIntro; lia.
+               }
+
+               iIntros "(Hown_frag & Hown_tok)".
+               wp_pures.
+               iModIntro; iApply "HΦ". 
+               iFrame "# ∗". iSplit; first done.
+               iRight. by iFrame "# ∗".
+          * iDestruct (own_valid_2 with "Hown_auth Hown_pred") 
+              as %[Hvalid%gset_included]%auth_both_valid_discrete.
+
+            rewrite (list_equiv_invert_L _ _ _ _ pred); last first.
+            { rewrite Hperm -elem_of_list_In elem_of_elements; set_solver. }
+
+            iDestruct "Hlist" as (? ? ? ? ?) "(_ & Hpt & #Hs & _ & _ & Hnode & _ & Himp)".
+            iDestruct "Hnode" as "(Hown_frag & Hown_tok)".
+            assert ({[ pred ]} = {[ pred ]} ⋅ {[ pred ]}) as -> by set_solver.
+            iDestruct "Hown_frag" as "(Hown_frag & Hown_frag_dup)".
+            assert ({[ pred ]} = {[ pred ]} ⋅ {[ pred ]}) as <- by set_solver.
+
+            wp_op.
+            iPoseProof ("Himp" $! {[ val_v dummy_val ]} dummy_val with "[Hpt Hown_frag_dup Hown_tok]") as "Hlist".
+            { iFrame; rewrite elem_of_singleton //. }
+            iMod ("Hclose" with "[Hlist Hown_auth Hown_toks]") as "_".
+            { iNext; iExists S', Smap', L; by iFrame. }
+            iModIntro.
+          
+            wp_bind (putAll _ _ _ _ _ _).
+            iApply ("IH" with "Hmatch [$] [%] [%]").
+            { lia. }
+            { lia. }
+
+            iNext. 
+            iIntros (opt n new) "(Hlist & Hopt)".
+            iDestruct "Hopt" as "[%Hopt | (%Hopt & Hown_frag & Hown_tok & Hown_key & %Hkey & #Hn & Hnext & Hlocks)]".
+            ++ rewrite Hopt; wp_pures.
+               iModIntro; iApply ("HΦ" $! _ n new).
+               iSplitR ""; last by iLeft.
+               by iFrame "# ∗".
+            ++ rewrite Hopt; wp_pures.
+
+               do 2 rewrite loc_add_assoc.
+               assert (Z.to_nat (h - (lvl - 1)) = S (Z.to_nat (h - lvl)))%nat as -> by lia.
+               assert (lvl - 1 + 1 = lvl) as -> by lia.
+               rewrite replicate_S ?array_cons.
+               iDestruct "Hnext" as "(Hnext' & Hnext)".
+               iDestruct "Hlocks" as "(Hlocks' & Hlocks)".
+
+               wp_apply (insert_spec _ _ _ new with "[Hown_frag Hown_tok Hnext' Hlocks']").
+               { rewrite Hkey //. }
+               { iFrame "# ∗"; iPureIntro; lia. }
+
+               iIntros "(Hown_frag & Hown_tok)".
+               wp_pures.
+               iModIntro; iApply "HΦ". 
+               iFrame "# ∗". iSplit; first done.
+               iRight. by iFrame "# ∗".
+    Qed.
+
+    Theorem put_spec (v: val) (key val ts height: Z) 
+      (Smap: gmap Z (argmax Z)) (q: frac) (bot: bot_gname) (subs: list sub_gname)
+      (Hrange: INT_MIN < key < INT_MAX) 
+      (Hheight: 0 ≤ height ≤ MAX_HEIGHT) :
+      {{{ is_skip_list v Smap q bot subs }}}
+        put v #key #val #ts #height
+      {{{ RET #(); is_skip_list v (Smap ⋅ {[ key := prodZ {[ val ]} ts ]}) q bot subs }}}.
+    Proof.
+      iIntros (Φ) "H HΦ".
+      iDestruct "H" as (h head) "(%Hv & Hpt & %Hmin & Hlist)".
+
+      wp_lam. wp_pures.
+      rewrite -Hv. wp_load. wp_let.
+
+      destruct subs as [|sub subs]; first by iExFalso.
+      wp_apply (topLevel_spec  with "[Hlist]").
+      { iFrame. iSplit; first by iLeft. iPureIntro; lia. }
+      iIntros (curr top_sub bot_subs).
+      iIntros "(Hlist & #Hown_curr & %Hcurr_range & Himp)".
+      wp_let.
+
+      wp_apply (putAll_spec with "[Hlist]").
+      { done. }
+      { iFrame "# ∗". iPureIntro; lia. }
+
+      iIntros (opt n new) "(Hlist & Hopt)".
+      iPoseProof ("Himp" with "Hlist") as "Hlist".
+      wp_let.
+
+      iModIntro; iApply "HΦ". 
+      iExists h, head. by iFrame.
+    Qed.
+
+  End Proofs.
+End AddSpec.
